# Computorv1

## Test Cases:

1. `x^2 + 5x + 6 = 0`
2. `X^2 - 16 = 0`
3. `X^2 + 2x + 1 = -3 + + 1`
4. `X^3 - 3X^2 + 3X + 1 = X^2 - 16`
5. `X^2 + 21=0+1`
6. `15 * 0 * 1 * 2 + X^2+ 1 =12*43         `
7. `1 + X^2 = 0 * - 1 + 2 + 1`
8. `3 * X^3 - 2 * X^2`
9. `3 * X^3 - 2 * X^2 + X^1 - 7 * X^0 = 2 * X^3 + 3 * X^2 - X^1 + 8 * X^0`
10. `5 * X^3 - 4 * X^2 + 2 * X^1 + 9 * X^0 = 4 * X^3 + 5 * X^2 - 3 * X^1 + 3 * X^0`
11. `6 * X^2 - 3 * X^1 + 8 * X^0 = X^2 + 4 * X^1 + 2 * X^0`
12. `4 * X^3 - 2 * X^2 + X^1 - 7 * X^0 = 2 * X^3 + 3 * X^2 - 4 * X^1 + 6 * X^0`
13. `4 * X^3 - 2 * X^2 + X^1 - 7 * X^0 = 2 * X^3 + 3 * X^2 - 4 * X^1 + 6 * X^0`
14. `7 * X^2 + 5 * X^1 - 2 * X^0 = 3 * X^3 + 6 * X^2 - 5 * X^1 - 9 * X^0`
15. `3 * X^3 + 4 * X^2 - 5 * X^1 + 2 * X^0 = 2 * X^3 - 4 * X^2 + 5 * X^1 - 2 * X^0`
16. `3 * X^3 + 4 * X^2 - 5 * X^1 + 2 * X^0 = 2 * X^3 - 4 * X^2 + 5 * X^1 - 2 * X^0`
17. `8 * X^3 - 6 * X^2 + 9 * X^0 = 4 * X^2 - 3 * X^1 + 7 * X^0`
18. `5 * X^3 + 3 * X^2 - X^1 + 2 * X^0 = 6 * X^3 + 4 * X^2 - 2 * X^1 + X^0`
19. `5 * X^3 + 3 * X^2 - X^1 + 2 * X^0 = 6 * X^3 + 4 * X^2 - 2 * X^1 + X^0`
20. `2 * X^3 - 4 * X^2 + X^1 + 7 * X^0 = X^2 - 6 * X^2 + 3 * X^1 + 2 * X^0`
21. `9 * X^3 - 3 * X^2 + 5 * X^1 - 2 * X^0 = 7 * X^3 - 4 * X^2 + 3 * X^1 + 9 * X^0`
22. `4 * X^2 - 7 * X^1 + 2 * X^0 = X^3 + 8 * X^2 - 2 * X^1 + 5 * X^0`
23. `3 * X^2 - 6 * X^1 + 1 * X^0 = 2 * X^3 + 7 * X^2 - 9 * X^1 + 5 * X^0`
24. `8 * X^3 - 5 * X^2 + 3 * X^1 + 6 * X^0 = 4 * X^3 - 2 * X^2 + 7 * X^1 + 9 * X^0`
25. `6 * X^3 - 8 * X^2 + 3 * X^1 - 2 * X^0 = 5 * X^3 - 9 * X^2 + 4 * X^1 - 6 * X^0`
26. `X^3 - 4 * X^2 + 3 * X^1 + 5 * X^0 = 3 * X^2 - 2 * X^1 + X^0`
27. `7 * X^3 + 3 * X^2 - X^0 = 5 * X^3 - 2 * X^2 + X^1 - 3 * X^0`
28. `5 * X^2 - 3 * X^1 + 4 * X^0 = 3 * X^3 + 4 * X^2 - 2 * X^1 + 6 * X^0`
29. `9 * X^3 - 2 * X^2 + 4 * X^1 - X^0 = 7 * X^3 + 5 * X^2 - 3 * X^1 + 9 * X^0`
30. `2 * X^3 - 3 * X^2 + X^1 - 5 * X^0 = 3 * X^3 + 4 * X^2 - 2 * X^1 + 7 * X^0`
31. `4 * X^3 + 3 * X^2 - 6 * X^1 + 7 * X^0 = X^3 + 5 * X^2 - 2 * X^1 + 8 * X^0`
32. `x^2 + 5x + 6 = 0`
33. `2 x^2 -4x + 1 =0`
34. `-3x^2+2x -5= 0`
35. `  4 * x^2 + 0*x + 0 =0`
36. `x^2 +0x - 16 =0`
37. `x^2-10x+25 = 0`
38. `-x^2 + x + 3=0`
39. `7x^2-2x+9=0`
40. `  x ^ 2 + x = 0`
41. `-8x^2 + 4x - 1 =0`
42. `   x^2+3 = 0`
43. `0*x^2 + 9*x + 4 = 0`
44. `  2x^2+3x+1= 0`
45. `9 *x^2 - 6 * x + 1 =0`
46. `-2x^2-4x-6 =0`
47. `x^2+ x +0=0`
48. `3*x^2+0*x+0 =0`
49. `1.5x^2 + 3.2x - 4.8 = 0`
50. `-x^2 - 2x - 1 = 0`
51. `100x^2 + 200x + 100 = 0`
52. `5x + 10 = 0`
53. `-2 * x + 3 = 0`
54. `0*x^2 + x - 7 = 0`
55. `x = 9`
56. `x + 0 = 0`
57. `x - 0= 0`
58. `10x - 100 = 0`
59. ` 3x + 2 = 0`
60. `-x + 5 = 0`
61. `x - 1.5 = 0`
62. `2.5x + 7.5 = 0`
63. `-7 * x + 0 = 0`
64. `0*x^2 + 6 * x + 0 = 0`
65. `x-3=0`
66. `x + 3.3 = 0`
67. `+1x + 2 = 0`
68. `-x + 0 = 0`
69. `0*x^2 - x = 0`
70. `2 * x = 0`
71. `x=0`
72. `9 = 0`
73. `  0 = 0`
74. `-5 = 0`
75. `   7   =    0`
76. `+4 = 0`
77. `-0.0001 = 0`
78. `100 = 0`
79. `-999 = 0`
80. `123456 = 0`
81. `-1 = 0`
82. `0.0 = 0`
83. `1e3 = 0`
84. `   +0 = 0`
85. `-000001 = 0`
86. `314 = 0`
87. `1 = 0`
88. `-3.14 = 0`
89. `-42 = 0`
90. `  2 = 0`
91. ` -8 = 0`
92. `x^2 + 3x + 2 = x^2 + 2x + 1`
93. `2x^2 + x + 1 = 0*x^2 + x + 1`
94. `3x^2 + 2x + 7 = 3x^2 + 2x + 7`
95. `x^2 - 4x + 4 = x^2 - 4x + 3`
96. `2x^2 +   2x + 1 = x^2 + x + 1`
97. `x^2 + x + 1 = 2x^2 + 2x + 2`
98. `x + 1 = 2x + 1`
99. `x = x`
100. `3x + 1 = 3x + 0`
101. `2x^2 + 2 = 2x^2 + 1`
102. `4x^2 + 4x = 4x^2 + 2x`
103. `x^2 = 2x`
104. `x^2 + x = x^2 + 1`
105. `3x = x + 2x`
106. `5x - 4 = 2x + 1`
107. `x^2 - x + 1 = 0`
108. `x^2 + 1 = x^2 + 1`
109. `2x^2 + 3x + 4 = 3x^2 + 2x + 5`
110. `x = 0.5x + 0.5x`
111. `x^2 + x + 1 = x^2 + 2x + 1`
112. `X^2 +2 * X + 1 = X^2 - 4*x + 4`
113. `5 *X^16 + 6 * X^12 = 0`
114. `x^999999=3`
115. `x^99=x^99-x`
116. `x^12=x+x^12+x^2-5`
117. `x^12=x+x^12"`
118. `x^12=x+x^12+x^2-5`
119. `x^12=x+x^12`
120. `x^12+x^2-4=x^12`
121. `x^99=x^99-x`
122. `x^12=5`
123. `5 *X^16 + 6 * X^12 = 0`
124. `5 *X^16`
125. `  4 * x^2 + 0*x + 0 =0"`
126. `-3*x^2+2*x -5= 0"`
127. `2*x^2 -4*x + 1 =0`
128. `x^2 + 5*x + 6 = 0`
129. `4 * X^3 - 2 * X^2 + X^1 - 7 * X^0 = 2 * X^3 + 3 * X^2 - 4 * X^1 + 6 * X^0`
130. `6 * X^2 - 3 * X^1 + 8 * X^0 = X^2 + 4 * X^1 + 2 * X^0`